src/Formalization/Examples/Example_Interval_Loop_Coverage.thy
@@ -36,7 +36,7 @@ subsection \<open>The compiled CFG\<close>
 abbreviation "loop_cfg \<equiv> compile_prog Map.empty [] loop_prog"
 
 lemma loop_cfg_full:
-  "loop_cfg = mk_ip_cfg 0 5
+  "loop_cfg = mk_cfg 0 5
      {(0, EA_Assign ''x'' (N 0), 1),
       (1, EA_Nop, 2),
       (2, EA_Assume (Less (V ''x'') (N 20)), 3),
@@ -80,13 +80,12 @@ definition loop_env :: "pp \<Rightarrow> ivl abs_state" where
       else (\<lambda>_. Ivl MinInf PlusInf))"
 
 lemma loop_postfix:
-  "is_post_fixpoint_ip loop_cfg ivl_tf (\<squnion>) bot loop_s0 loop_env"
-  unfolding is_post_fixpoint_ip_def
+  "is_post_fixpoint loop_cfg ivl_tf (\<squnion>) bot loop_s0 loop_env"
+  unfolding is_post_fixpoint_def
 proof (rule allI)
   fix v
-  show "rhs_ip loop_cfg ivl_tf (\<squnion>) bot loop_s0 loop_env v \<le> loop_env v"
-    apply (simp only: rhs_ip_eq_rhs_if_no_combines[OF loop_cfg_combines]
-                      rhs_def Let_def loop_cfg_entry loop_cfg_edges)
+  show "rhs loop_cfg ivl_tf (\<squnion>) bot loop_s0 loop_env v \<le> loop_env v"
+    apply (simp only: rhs_def Let_def loop_cfg_entry loop_cfg_edges loop_cfg_combines)
     apply (rule abs_join_set_le)
     apply (rule finite_subset[where B=
             "insert loop_s0 ((\<lambda>(u,a). apply_tf ivl_tf a (loop_env u)) `
@@ -108,7 +107,7 @@ abbreviation "loop_head \<equiv> 2"
 
 lemma loop_head_x_bounded:
   assumes S_sound: "S \<subseteq> ivl_domain.gamma_state loop_s0"
-  assumes tr: "tr \<in> cfg_collect_trace_ip loop_cfg S loop_head"
+  assumes tr: "tr \<in> cfg_collect_trace loop_cfg S loop_head"
   shows "0 \<le> (last tr) ''x'' \<and> (last tr) ''x'' \<le> 20"
 proof -
   have fin_e: "finite (edges loop_cfg)" by (simp add: loop_cfg_edges)
