src/Formalization/Examples/Example_Interval_Side_Proc_Global.thy
@@ -1,13 +1,13 @@
 section \<open>Example: TD\_side Interval Analysis on a Single Global Increment Call\<close>
 
 theory Example_Interval_Side_Proc_Global
-  imports "Voblint_Analysis.Interval_Side_IP_Soundness" "Voblint_CFG.CFG_Collect_IP_Adeq"
+  imports "Voblint_Analysis.Interval_Side_Soundness" "Voblint_CFG.CFG_Collect_Adeq"
 begin
 
 text \<open>
   Interval instance of the side-effecting interprocedural witness: the same
   @{const inc_pi} program (a single call to procedure p incrementing the global
-  @{term \<open>''Gx''\<close>}) carried through the @{const side_analyse_ip_eff} solver at the
+  @{term \<open>''Gx''\<close>}) carried through the @{const side_analyse_eff} solver at the
   interval domain.  Demonstrates the soundness scaffold is domain-generic by
   reusing it on a second, infinite-height numeric domain.
 \<close>
@@ -22,22 +22,22 @@ definition side_proc_global_ivl_s0 :: "ivl abs_state" where
 theorem proc_global_side_ivl_analysis:
   fixes s t :: store
   assumes s_sound: "s \<in> ivl_domain.gamma_state side_proc_global_ivl_s0"
-  assumes runs: "pruns_to_ip inc_pi [''p''] (Call ''p'') s t"
+  assumes runs: "cfg_runs_to inc_pi [''p''] (Call ''p'') s t"
   assumes side_solve_dom:
-    "side_cfg_ip_solve_dom_eff (compile_prog inc_pi [''p''] (Call ''p'')) ivl_etf bot
+    "side_cfg_solve_dom_eff (compile_prog inc_pi [''p''] (Call ''p'')) ivl_etf bot
        side_proc_global_ivl_s0
        (cfg_exit (compile_prog inc_pi [''p''] (Call ''p'')))"
   shows "t \<in> ivl_domain.gamma_state
-       (side_analyse_ip_eff inc_pi [''p''] (Call ''p'') ivl_etf bot side_proc_global_ivl_s0
+       (side_analyse_eff inc_pi [''p''] (Call ''p'') ivl_etf bot side_proc_global_ivl_s0
          (cfg_exit (compile_prog inc_pi [''p''] (Call ''p''))))"
 proof -
   have collect_exit:
-    "t \<in> cfg_collect_ip (compile_prog inc_pi [''p''] (Call ''p'')) {s}
+    "t \<in> cfg_collect (compile_prog inc_pi [''p''] (Call ''p'')) {s}
        (cfg_exit (compile_prog inc_pi [''p''] (Call ''p'')))"
-    using runs unfolding pruns_to_ip_def
+    using runs unfolding cfg_runs_to_def
     by (metis singleton_store_def)
   show ?thesis
-    by (rule side_ip_ivl_analysis_sound[OF s_sound collect_exit side_solve_dom])
+    by (rule side_ivl_analysis_sound[OF s_sound collect_exit side_solve_dom])
 qed
 
 end
