src/Formalization/Examples/Example_Side_Proc_Global.thy
@@ -2,15 +2,15 @@ section \<open>Example: TD\_side Sign Analysis on a Single Global Increment Call
 
 theory Example_Side_Proc_Global
   imports
-    "Voblint_Analysis.Sign_Side_IP_Soundness"
+    "Voblint_Analysis.Sign_Side_Soundness"
     "Voblint_Analysis.Sign_Exec_Sound"
-    "Voblint_CFG.CFG_Collect_IP_Adeq"
+    "Voblint_CFG.CFG_Collect_Adeq"
 begin
 
 text \<open>
   Side-effecting interprocedural witness: @{const inc_pi} with a single call to
-  procedure p.  Operational semantics via @{const pruns_to_ip}; soundness via
-  @{const side_analyse_ip_eff} (the effectful side TD solver).
+  procedure p.  Operational semantics via @{const cfg_runs_to}; soundness via
+  @{const side_analyse_eff} (the effectful side TD solver).
 \<close>
 
 (* A non-trivial initial state: every variable -- including the globals --
@@ -23,22 +23,22 @@ definition side_proc_global_s0 :: "sign abs_state" where
 theorem proc_global_side_sign_analysis:
   fixes s t :: store
   assumes s_sound: "s \<in> sign_domain.gamma_state side_proc_global_s0"
-  assumes runs: "pruns_to_ip inc_pi [''p''] (Call ''p'') s t"
+  assumes runs: "cfg_runs_to inc_pi [''p''] (Call ''p'') s t"
   assumes side_solve_dom:
-    "side_cfg_ip_solve_dom_eff (compile_prog inc_pi [''p''] (Call ''p'')) sign_etf bot
+    "side_cfg_solve_dom_eff (compile_prog inc_pi [''p''] (Call ''p'')) sign_etf bot
        side_proc_global_s0
        (cfg_exit (compile_prog inc_pi [''p''] (Call ''p'')))"
   shows "t \<in> sign_domain.gamma_state
-       (side_analyse_ip_eff inc_pi [''p''] (Call ''p'') sign_etf bot side_proc_global_s0
+       (side_analyse_eff inc_pi [''p''] (Call ''p'') sign_etf bot side_proc_global_s0
          (cfg_exit (compile_prog inc_pi [''p''] (Call ''p''))))"
 proof -
   have collect_exit:
-    "t \<in> cfg_collect_ip (compile_prog inc_pi [''p''] (Call ''p'')) {s}
+    "t \<in> cfg_collect (compile_prog inc_pi [''p''] (Call ''p'')) {s}
        (cfg_exit (compile_prog inc_pi [''p''] (Call ''p'')))"
-    using runs unfolding pruns_to_ip_def
+    using runs unfolding cfg_runs_to_def
     by (metis singleton_store_def)
   show ?thesis
-    by (rule side_ip_sign_analysis_sound[OF s_sound collect_exit side_solve_dom])
+    by (rule side_sign_analysis_sound[OF s_sound collect_exit side_solve_dom])
 qed
 
 subsection \<open>Executable sign analysis\<close>
@@ -63,7 +63,7 @@ lemma inc_terminates: "sign_terminates_prog inc_prog"
   by (rule sign_terminates_prog_via_solve_c) eval
 
 corollary inc_certified_sound:
-  "cfg_collect_ip (prog_cfg inc_prog) cinit_stores (cfg_exit (prog_cfg inc_prog))
+  "cfg_collect (prog_cfg inc_prog) cinit_stores (cfg_exit (prog_cfg inc_prog))
    \<le> sign_domain.gamma_state (sign_exec_prog inc_prog)"
   by (rule sign_exec_prog_sound_collecting[OF inc_terminates])
 
